---
title:      Exercise 3.2-7
published:  2012-08-25 19:30
modified:   2020-10-12 22:30
redirect_from:
  - /E03.02-07/
keywords:    "Fibonacci number, Fibonacci conjugate"
description: "Prove by induction that the i-th Fibonacci number satisfies the equality... where ϕ is the golden ratio and ϕ^​ is its conjugate."
---

> Prove by induction that the $$i$$-th Fibonacci number satisfies the equality
>
> $$F_i = \frac {\phi^i - \hat{\phi^i}} {\sqrt 5}$$
>
> where $$\phi$$ is the golden ratio and $$\hat\phi$$ is its conjugate.

From chapter text, the values of $$\phi$$ and $$\hat\phi$$ are as follows:

$$\phi = \frac {1 + \sqrt 5} 2 \qquad \hat\phi = \frac {1 - \sqrt 5} 2$$

And, Fibonacci series is defined by:

$$\begin {aligned}
F_i = \begin {cases}
    0 & \text { for } i = 0 \\
    1 & \text { for } i = 1 \\
    F_{i-1} + F_{i-2} & \text { for } i \ge 2
\end {cases}
\end {aligned}$$

#### Base Case

We need to show the equality holds for both $$i = 0$$ and $$i = 1$$.

$$\begin {aligned}
F_0 & = \frac {\phi^0 - \hat\phi^0} {\sqrt 5} = \frac {1 - 1} {\sqrt 5} = 0 \\[2ex]
F_1 & = \frac {\phi^1 - \hat\phi^1} {\sqrt 5} = \frac {\sqrt 5} {\sqrt 5} = 1
\end {aligned}$$

#### Inductive Step

Let us assume that the equality holds for $$i = k$$ and $$i = k - 1$$ such that $$k \ge 2$$. We have to show that it holds for $$i = k + 1$$ too.

$$\begin {aligned}
F_{k + 1} & = F_k + F_{k - 1} \\
          & = \frac {\phi^k - \hat\phi^k} {\sqrt 5} + \frac {\phi^{k - 1} - \hat\phi^{k - 1}} {\sqrt 5} \\
          & = \frac {(\phi^k - \hat\phi^k) + (\phi^{k - 1} - \hat\phi^{k - 1})} {\sqrt 5} \\
          & = \frac {(\phi^k + \phi^{k - 1}) - (\hat\phi^k + \hat\phi^{k - 1})} {\sqrt 5} \\
          & = \frac {\phi^{k - 1}(\phi + 1) - \hat\phi^{k - 1}(\hat\phi + 1)} {\sqrt 5}\\
          & = \frac {\phi^{k - 1}\cdot\phi^2 - \hat\phi^{k - 1}\cdot\hat\phi^2} {\sqrt 5}\\
          & = \frac {\phi^{k + 1} - \hat\phi^{k + 1}} {\sqrt 5}
\end {aligned}$$

So, the inequality holds for $$k + 1$$ also.
Hence, the proof is complete.

{% capture note %}
We are using the property that $$\phi + 1 = \phi^2$$ and $$\hat\phi + 1 = \hat\phi^2$$ in this proof, which is already shown in the [previous exercise]({% link _solutions/03/E03.02-06.md %}){:target="_blank"}.
{% endcapture %}
{% include aside.html title="In case you missed it ..." %}
