---
title:      Exercise 3.2-2
clrs:       [3, 2]
published:  2012-08-25 19:05
modified:   2020-10-12 22:30
---

> Prove equation (3.16).

Equation 3.16 says: $$a^{\log_b c} = c^{\log_b a}$$

This can be shown in many ways, all of which requires rewriting and manipulating logarithmic identities that were listed in the book just before equation 3.16.

##### Method 1

$$\begin {aligned}
a^{\log_b c} & = (b^{\log_b a})^{\log_b c} \\
             & = (b^{\log_b c})^{\log_b a} \\
             & = c^{\log_b a}
\end {aligned}$$

##### Method 2

$$\begin {aligned}
a^{\log_b c} & = a^{\log_a c/\log_a b} \\
             & = \big(a^{\log_a c}\big)^{1 / {\log_a b}} \\
             & = c^{1 / {\log_a b}} \\
             & = c^{\log_b a}
\end {aligned}$$
