---
title:      Exercise 3.2-6
clrs:       [3, 2]
published:  2012-08-25 19:25
modified:   2020-10-12 22:30
---

> Show that the golden ratio $$\phi$$ and its conjugate $$\hat\phi$$ both satisfy the equation $$x^2 = x + 1$$.

$$\begin {aligned}
\phi^2 & = \left(\frac {1 + \sqrt 5} 2\right)^2 \\
       & = \frac {1 + 2\sqrt 5 + 5} 4 \\
       & = \frac {3 + \sqrt 5} 2 \\
       & = \frac {1 + \sqrt 5} 2 + 1 \\
       & = \phi + 1
\end {aligned}$$

$$\begin {aligned}
\hat{\phi^2} & = \left(\frac {1 - \sqrt 5} 2\right)^2 \\
             & = \frac {1 - 2\sqrt 5 + 5} 4 \\
             & = \frac {3 - \sqrt 5} 2 \\
             & = \frac {1 - \sqrt 5} 2 + 1 \\
             & = \hat\phi + 1
\end {aligned}$$

{% capture note %}
We can also show this proof, by finding solutions to the given quadratic equation, $$x^2 - x - 1 = 0$$. Which will be equal to $$\phi$$ and $$\hat\phi$$.
{% endcapture %}
{% include aside.html title="Doing it in reverse" %}
