---
title:      Exercise 4.4-5
published:  2012-08-28 21:15
modified:   2021-02-08 21:10
redirect_from:
  - /E04.04-05/
keywords:    "recursion tree, substitution method"
description: "Use a recursion tree to determine a good asymptotic upper bound on the recurrence T(n) = T(nâˆ’1) + T(n/2) + n. Use the substitution method to verify your answer."
---

> Use a recursion tree to determine a good asymptotic upper bound on the recurrence $$T(n) = T(n - 1) + T(n/2) + n$$. Use the substitution method to verify your answer.

{% capture note %}
[_January 2021_] The earlier version of the solution was completely wrong and most of the comments refer to that. The solution has since been updated. Please do not get confused by old comments.
{% endcapture %}
{% include aside.html title='Note About Comments' %}

This problem is pretty interesting and at the same time quite difficult.

Also I'll deviate from my usual approach of solving earlier exercises in this chapter, as there are two branches at each level of this recurrence which grows quite differently.

Getting an upper bound is easy, as we can find a recurrence that definitely grows much faster than this one. But finding a tight upper bound is tricky.

{% capture note %}
Usually in the book as well as in your course work when upper bound is talked about, it always means tight upper bound. What is the difference?

Let's say, $$f(n) = n$$. A tight upper bound for $$f$$ will be $$O(n)$$. However, $$O(n^2)$$, $$O(n^3)$$ etc. are also upper bounds of $$f$$, as $$f$$ will be asymptotically smaller than functions like $$n^2$$, $$n^3$$ etc.
{% endcapture %}
{% include aside.html title='Upper Bound vs Tight Upper Bound' %}

#### Just An Upper Bound

Note that, asymptotically,

$$T(n) = T(n - 1) + T(n/2) + n \le 2T(n - 1) + n$$

And the above holds as long as we choose $$n \ge 2$$.

Now the recurrence tree for the larger recurrence (the right one) of the above:

Rate of increase in number of subproblems in each recursion = 2

Rate of decrease in subproblem size = 1 with 1 less input

Hence at depth $$i = 0, 1, 2, \dots, n$$ of the tree, there are $$2^i$$ nodes each of cost $$(n - i)$$.

Hence, total cost of the tree is:

$$\begin {aligned}
T(n) & = \sum_{i = 0}^{n} 2^i \cdot (n - i) \\
     & = n\sum_{i = 0}^{n} 2^i - \textcolor {blue} {\sum_{i = 0}^{n} i \cdot 2^i}
\end {aligned}$$

The second sum in the above equation (highlighted in blue) can be computed in [many ways](https://math.stackexchange.com/questions/11464/how-to-compute-the-formula-sum-limits-r-1d-r-cdot-2r){:target="_blank"}. Here is one such method:

$$\begin {aligned}
     S &= 1 \cdot 2^1 + &&2 \cdot 2^2 + \cdots + &(n - 1)& \cdot 2^{n - 1} + &n& \cdot 2^n  \\
    2S &=               &&1 \cdot 2^2 + \cdots + &(n - 2)& \cdot 2^{n - 1} + &(n - 1)& \cdot 2^n &&+ n \cdot 2^{n + 1} \\
S - 2S &= 1 \cdot 2^1 + &&1 \cdot 2^2 + \cdots + &1& \cdot 2^{n - 1} + &1& \cdot 2^n &&- n \cdot 2^{n + 1}
\end {aligned}$$

Simplifying further:

$$\begin {aligned}
S &= n \cdot 2^{n + 1} - (2^1 + 2^2 + \cdots + 2^n) \\
  &= n \cdot 2^{n + 1} - (2^0 + 2^1 + 2^2 + \cdots + 2^n) + 2^0 \\
  &= n \cdot 2^{n + 1} - \sum_{i = 0}^{n} 2^i + 1 \\
\end {aligned}$$

Going back to our recurrence cost:

$$\begin {aligned}
T(n) & = \sum_{i = 0}^{n} 2^i \cdot (n - i) \\
     & = n\sum_{i = 0}^{n} 2^i - \textcolor {blue} {\sum_{i = 0}^{n} i \cdot 2^i} \\
     & = n\sum_{i = 0}^{n} 2^i - \textcolor {blue} {\left(n \cdot 2^{n + 1} - \sum_{i = 0}^{n} 2^i + 1\right)} \\
     & = (n + 1) \cdot \sum_{i = 0}^{n} 2^i - n \cdot 2^{n + 1} - 1 \\
     & = (n + 1) \cdot \frac {2^{n + 1} - 1} {2 - 1} - n \cdot 2^{n + 1} - 1 \\
     & = (n + 1) \cdot (2^{n + 1} - 1) - n \cdot 2^{n + 1} - 1 \\
     & = n \cdot 2^{n + 1} - n + 2^{n + 1} - 1 - n \cdot 2^{n + 1} - 1 \\
     & = 2^{n + 1} - n - 2 \\
     & \le 2^{n + 1} \\
     & \le c2^n \\
\end {aligned}$$

The last step holds as long as $$c \ge 2$$ and $$n \ge 0$$.

So, $$T(n)$$ is definitely $$O(2^n)$$ and we can use this as an initial guess to show this holds true using the substitution method.

{% capture note %}
As I mentioned earlier, the above approach only gives an upper bound, but we did not show a tight upper bound. In fact the tight upper bound of the above problem is somewhere between $$O(n^2)$$ and $$O(2^n)$$.

Check out [this post](https://math.stackexchange.com/a/518859){:target="_blank"} in the Mathematics Stack Exchange forum which discusses many guesses, and finally settles down with $$O(n^{\lg n})$$.
{% endcapture %}
{% include aside.html title='What about tight upper bound' %}
