---
title:       Exercise 4.3-1
published:   2012-08-28 20:00
modified:    2021-01-26 10:30
keywords:    "recurrence, substitution"
description: "Show that the solution of T(n) = T(n−1) + n is O(n²)."
---

> Show that the solution of $$T(n) = T(n - 1) + n$$ is $$O(n^2)$$.

Let us assume $$T(n) \le cn^2$$ for all $$n \ge n_0$$, where $$c$$ and $$n_0$$ are positive constants. We'll specify the constants later based on our induction requirements.

Hence, $$T(n - 1) \leq c(n - 1)^2$$

Therefore, we can write:

$$\begin {aligned}
T(n) & \le c(n - 1)^2 + n \\
     & = cn^2 - 2cn + c + n \\
     & = cn^2 - (n(2c - 1) - c) \\
     & \le cn^2
\end {aligned}$$

The last step holds as long as $$(n(2c - 1) - c) \ge 0$$. We can use this to specify $$c$$ and $$n_0$$.

If we pick $$c = 1$$, then we need $$n - 1 \ge 0$$. Which is possible as long as $$n \ge 1 = n_0$$.

{% include ads.html %}

#### Solving Without Substitution

This particular problem can be solved using a much simpler method, that does not use substitution.

We can safely assume $$T(0) = k$$, where $$k$$ is positive constant, as for input size zero we need to do only a constant amount of work, e.g. checking input size and returning.

Therefore:

$$\begin{aligned}
T(1) &= T(0) + 1 = k + 1 \\
T(2) &= T(1) + 2 = k + 1 + 2 \\
T(3) &= T(2) + 3 = k + 1 + 2 + 3 \\
\cdots \\
T(n) &= T(n - 1) + n = k + 1 + 2 + 3 + \cdots + n \\
     &= k + \frac {n(n + 1)} 2 \\
     &= \Theta(n^2)
\end{aligned}$$
