---
title:      Exercise 4.3-2
published:  2012-08-28 20:05
modified:   2021-01-21 10:30
redirect_from:
  - /E04.03-02/
keywords:    "recurrence, substitution"
description: "Show that the solution of T(n) = T(⌈n/2⌉) + 1 is O(lg⁡ n)."
---

> Show that the solution of $$T(n) = T(\lceil n / 2 \rceil) + 1$$ is $$O(\lg n)$$.

Let us assume $$T(n) \le c \lg n$$ for all $$n \ge n_0$$, where $$c$$ and $$n_0$$ are positive constants.

$$\begin {aligned}
T(n) & \le c \lg \left \lceil \frac n 2 \right \rceil + 1 \\
     & < c \lg \left( \frac n 2 + 1 \right) + 1 \\
     & < c \lg \left( \frac {n + 2} 2 \right) + 1 \\
     & = c \lg (n + 2) - c \lg 2 + 1 \\
     & = c \lg (n + 2) - c + 1
\end {aligned}$$

This is inconclusive, as we cannot arrive at our assumption from the last step. So we'll modify our assumption a bit by subtracting a lower-order term from our previous guess.

Let us assume $$T(n) \le c \lg (n - 2)$$.

$$\begin {aligned}
T(n) & \le c \lg \left \lceil \frac n 2 - 2\right \rceil + 1 \\
     & < c \lg \left( \frac n 2 - 2 + 1 \right) + 1 \\
     & < c \lg \left( \frac {n - 2} 2 \right) + 1 \\
     & = c \lg (n - 2) - c \lg 2 + 1 \\
     & = c \lg (n - 2) - (c - 1) \\
     & \le c \lg (n - 2)
\end {aligned}$$

The last step holds as long as $$c \ge 1$$.

{% capture note %}
The clue to picking the _lower-order term_ is actually in our unsuccessful attempt. In the first guess, we ended up with $$cn \lg (n + 2)$$ instead of desired $$cn \lg n$$. So we are basically trying to remove the additional 2. So subtracting 2 from our initial guess should work as a modified guess.

And note this pattern for subtracting/adding 2 whenever ceiling/floor functions are involved. We'll use this repeatedly.
{% endcapture %}
{% include aside.html title='Why We Chose 2' %}