---
title:      Exercise 4.3-3
clrs:       [4, 3]
published:  2012-08-28 20:10
modified:   2021-01-21 10:30
---

> We saw that the solution of $$T(n) = 2T(\lfloor n/2 \rfloor) + n$$ is $$O(n \lg n)$$. Show that the solution of this recurrence is also $$\Omega(n \lg n)$$. Conclude that the solution is $$\Theta(n \lg n)$$.

To show $$T(n) = \Omega(n \lg n)$$, we need to show $$T(n) \ge c n \lg n$$, for all $$n \ge n_0$$,  where $$c$$ and $$n_0$$ are some positive constants.

Let's assume, $$T(n) \ge c n \lg n$$, and it holds for all positive $$m < n$$, in particular for $$m = \lfloor n/2 \rfloor$$.

$$\begin {aligned}
T(n) &= 2T(\lfloor n/2 \rfloor) + n \\
     &\ge 2 c \lfloor n/2 \rfloor \lg \lfloor n/2 \rfloor + n \\
     &\ge 2 c (n/2 - 1) \lg (n/2 - 1) + n \\
     &= 2 c \left(\frac {n - 2} 2\right) \lg \left(\frac {n - 2} 2\right) + n \\
     &= c(n - 2) \lg (n - 2) - c(n - 2) \lg 2 + n \\
     &= c(n - 2) \lg (n - 2) + (1 - c)n + 2c \\
\end {aligned}$$

As in previous [exercise]({% link _solutions/04/E04.03-02.md %}#why-we-chose-2){:target='_blank'}, this is inconclusive, and we need to compensate for the $$-2$$ term. We'll do that by modifying our previous guess, by _adding_ 2 our initial guess.

Let's assume, $$T(n) \ge c (n + 2) \lg (n + 2)$$

$$\begin {aligned}
T(n) &\ge 2 c (\lfloor n/2 \rfloor + 2) \lg (\lfloor n/2 \rfloor + 2) + n \\
     &\ge 2 c (n/2 - 1 + 2) \lg (n/2 - 1 + 2) + n \\
     &= 2 c \left(\frac {n + 2} 2\right) \lg \left(\frac {n + 2} 2\right) + n \\
     &= c(n + 2) \lg (n + 2) - c(n + 2) \lg 2 + n \\
     &= c(n + 2) \lg (n + 2) + \textcolor {blue} {(1 - c)n - 2c} \\
     &\ge c(n + 2) \lg (n + 2) \\
\end {aligned}$$

The last step holds as long as the term marked in blue is positive, i.e. $$n \ge \frac {2c}{1 - c}$$.

Hence, we need $$0 \le c < 1$$.

If we pick $$c = 0$$, then our assumption holds for $$n \ge 0 = n_0$$.

If we pick $$c = 1/2$$, then our assumption holds for $$n \ge 2 = n_0$$.
