---
title:       Exercise 4.3-5
published:   2012-08-28 20:20
modified:    2021-01-21 10:30
keywords:    "recurrence, substitution"
description: "Show that Θ(nlg⁡n) is the solution to the “exact” recurrence (4.3) for merge sort."
---

> Show that $$\Theta(n \lg n)$$ is the solution to the "exact" recurrence (4.3) for merge sort.

The recurrence (4.3) is given by:

$$
T(n) =
\begin{cases}
    \Theta(1)                                                 & \text{if $n = 1$,} \\
    T(\lceil n/2 \rceil) + T(\lfloor n/2 \rfloor) + \Theta(n) & \text{if $n > 1$.} \\
\end{cases}
$$

To show $$\Theta$$ bound, we need to separately show $$O$$ and $$\Omega$$ bounds.

Let us assume, $$\Theta(n) = kn$$ for the recurrence stated above, where $$k$$ is a positive constant.

#### O Bound

Let us assume $$T(n) \le c (n - 2) \lg (n - 2)$$ for all $$n \ge n_0$$, for some positive constants $$c$$ and $$n_0$$. [[Why subtract 2]({% link _solutions/04/E04.03-02.md %}#why-we-chose-2){:target='_blank'}]

$$\begin {aligned}
T(n) &= T(\lceil n/2 \rceil) + T(\lfloor n/2 \rfloor) + kn \\
     &\le c(\lceil n/2 \rceil - 2) \lg (\lceil n/2 \rceil - 2) + c(\lfloor n/2 \rfloor - 2) \lg (\lfloor n/2 \rfloor - 2) + kn \\
     &\le c (n/2 + 1 - 2) \lg (n/2 + 1 - 2) + c (n/2 + 1 - 2) \lg (n/2 + 1 - 2) + kn \\
     &= 2c (n/2 - 1) \lg (n/2 - 1) + kn \\
     &= c (n - 2) \lg (n - 2)/2 + kn \\
     &= c (n - 2) \lg (n - 2) - c (n - 2) \lg 2 + kn \\
     &= c (n - 2) \lg (n - 2) - c (n - 2) + kn \\
     &= c (n - 2) \lg (n - 2) - ((c - k)n - 2c) \\
     &\le c (n - 2) \lg (n - 2) \\
\end{aligned}$$

The last step holds as long as $$((c - k)n - 2c) > 0$$.

Therefore, we can pick $$c \ge k$$ and $$n \ge n_0 = \frac {2c} {c - k}$$.

**Note:** In the 3rd line of the above derivation, we used the fact that both $$\lfloor n \rfloor$$ and $$\lceil n \rceil$$ are less than $$n + 1$$.

{% include ads.html %}

#### Ω Bound

Let us assume $$T(n) \ge d (n + 2) \lg (n + 2)$$ for all $$n \ge n_0$$, for some positive constants $$d$$ and $$n_0$$. [[Why add 2]({% link _solutions/04/E04.03-02.md %}#why-we-chose-2){:target='_blank'}]

$$\begin {aligned}
T(n) &= T(\lceil n/2 \rceil) + T(\lfloor n/2 \rfloor) + kn \\
     &\ge d(\lceil n/2 \rceil + 2) \lg (\lceil n/2 \rceil + 2) + d(\lfloor n/2 \rfloor + 2) \lg (\lfloor n/2 \rfloor + 2) + kn \\
     &\ge d (n/2 - 1 + 2) \lg (n/2 - 1 + 2) + d (n/2 - 1 + 2) \lg (n/2 - 1 + 2) + kn \\
     &= 2d (n/2 + 1) \lg (n/2 + 1) + kn \\
     &= d (n + 2) \lg (n + 2)/2 + kn \\
     &= d (n + 2) \lg (n + 2) - d (n + 2) \lg 2 + kn \\
     &= d (n + 2) \lg (n + 2) - d (n + 2) + kn \\
     &= d (n + 2) \lg (n + 2) + ((k - d)n - 2d) \\
     &\ge d (n + 2) \lg (n + 2) \\
\end{aligned}$$

The last step holds as long as $$((k - d)n - 2d) > 0$$.

Therefore, we can pick $$d \le k$$ and $$n \ge n_0 = \frac {2d} {k - d}$$.

**Note:** In the 3rd line of the above derivation, we used the fact that both $$\lfloor n \rfloor$$ and $$\lceil n \rceil$$ are greater than $$n - 1$$.

{% capture note %}
If you note, I have skipped showing how the boundary condition is met for these assumptions. We can show it by setting the boundary condition for inductive proof at a much higher value of $$n_0$$. And from there work backward to match it with the boundary condition of the recurrence, which is  set at $$n = 1$$.

This is how it has been discussed in the book (page 84 in 3rd edition).
{% endcapture %}
{% include aside.html title='What about boundary condition' %}
