---
title:       Exercise 4.3-9
published:   2012-08-28 20:40
modified:    2021-01-21 10:30
keywords:    "recurrence substitution, change of variables"
description: "Solve the recurrence T(n) = 3T(√n) + log⁡n by making a change of variables. Your solution should be asymptotically tight. Do not worry about whether values are integral."
---

> Solve the recurrence $$T(n) = 3T(\sqrt n) + \log n$$. by making a change of variables. Your solution should be asymptotically tight. Do not worry about whether values are integral.

**Note:** I don't why suddenly $$\log$$ is used in this problem statement, whereas till now everywhere $$\lg$$ was used. I'm assuming in this context, $$\log$$ still means $$\log_2 = \lg$$.

Let us assume $$n = 2^m$$, $$m = \lg n$$.

Hence, the recurrence takes the form

$$T(2^m) = 3T(2^{m/2}) + m$$.

Now, assuming $$S(m) = T(2^m)$$, the recurrence takes the form

$$S(m) = 3S(m/2) + m$$.

{% capture note %}
If you are not reading ahead and don't know Master theorem yet, it'll be really difficult to make good initial guess here. However, as a reader has pointed out in the [comments section](#disqus_thread), we can identify a pattern in the solutions for recurrence relation.

If a recurrence is given by $$T(n) = aT(n / b) + f(n)$$, the solutions are usually of the form $$O(n^{log_b a})$$. This is heavily simplified, but nevertheless a good intuitive deduction. And you'll see that Master theorem states similar solution under certain conditions.
{% endcapture %}
{% include aside.html title='What Can We Guess' %}

{% include ads.html %}

Let's assume, $$S(m) \le cm^{\lg 3}$$, for all $$m \ge m_0$$, where $$c$$ and $$m_0$$ are some positive constants.

$$\begin {aligned}
S(m) & = 3S(m/2) + m \\
     & \le 3c(m/2)^{\lg 3} + m \\
     & = 3c \frac {m^{\lg 3}} {2^{\lg 3}} + m \\
     & = cm^{\lg 3} + m
\end {aligned}$$

With this we cannot prove our assumption in it's exact form.

So, let us modify our assumption by subtracting  a lower-order term.

Let's assume $$S(m) \le cm^{\lg 3} - bm$$.

$$\begin {aligned}
S(m) & = 3S(m/2) + m \\
     & \le 3(c(m/2)^{\lg 3} - b(m/2)) + m \\
     & = 3c \frac {m^{\lg 3}} {2^{\lg 3}} - 3bm/2 + m \\
     & = cm^{\lg 3} - bm - (b/2 - 1)m \\
     & \le cm^{\lg 3} - bm
\end {aligned}$$

The last step holds as long as $$(b/2 - 1)m$$ is positive.

If we set $$m_0 = 1$$, we need $$b \ge 2$$.

Changing our variable back to $$n$$, we have:

$$T(n) = O(m^{\lg 3}) = O((\lg n)^{\lg 3}) = O(\lg^{\lg 3} n)$$

{% capture note %}
We can similarly show the $$\Theta$$ bound as well. In fact, our first inductive hypothesis, which failed to prove $$O$$ bound, can be used directly to show the $$\Omega$$ bound. Both together proves the $$\Theta$$ bound.
{% endcapture %}
{% include aside.html title='What about Θ Bound' %}
